Spacetalk/Compiler.lean
@@ -1,0 +1,80 @@
+import Spacetalk.Arith
+import Spacetalk.DF
+
+open Arith DF
+
+namespace Compiler
+
+structure MarkedDFG where
+  dfg : DFG
+  ret : Port
+
+-- Merge consumers of input nodes that map to the same variable
+@[simp]
+def mergeVarsAux (dfg : DFG) (node : Node) : DFG :=
+  match node with
+  | ⟨_, .input var newPorts⟩ =>
+    let idx := dfg.findIdx
+      (λ node =>
+        match node with
+        | ⟨_, .input var' _⟩ => var' = var
+        | _ => false
+      )
+    match dfg.get? idx with
+    | some ⟨nid, .input var ports⟩ =>
+      dfg.set idx ⟨nid, .input var (ports ++ newPorts)⟩
+    | _ => node :: dfg
+  | _ => node :: dfg
+
+@[simp]
+def mergeVars (g1 g2 : DFG) : DFG :=
+  g2.foldl mergeVarsAux g1
+
+-- Update the "return" value of a graph to be the port of the new output node
+@[simp]
+def updateReturn (dfg : DFG) (ret : Port) (newRet : Port) :=
+  dfg.map
+    (λ node =>
+      let replace (p : Port) := if p = ret then newRet else p
+      {node with op :=
+        match node.op with
+        | .input var ports => .input var (ports.map replace)
+        | .output => .output
+        | .binOp op ports => .binOp op (ports.map replace)
+      }
+    )
+
+@[simp]
+def removeOutputNodes (dfg : DFG) : DFG :=
+  dfg.filter (λ node => match node.op with | .output => false | _ => true)
+
+@[simp]
+def mergeTwo (g1 g2 : MarkedDFG) (newOutput : Nat)
+  : DFG :=
+  let dfg := mergeVars g1.dfg g2.dfg
+  -- Update links to the original output nodes
+  let dfg := updateReturn dfg g1.ret ⟨newOutput, 0⟩
+  let dfg := updateReturn dfg g2.ret ⟨newOutput, 1⟩
+  removeOutputNodes dfg
+
+@[simp]
+def compileAux (maxNid : Nat) : Exp → MarkedDFG × Nat
+  | .var var =>
+    let inpId := maxNid
+    let outId := maxNid + 1
+    let dfg := [⟨inpId, .input var [⟨outId, 0⟩]⟩, ⟨outId, .output⟩]
+    (⟨dfg, ⟨outId, 0⟩⟩, maxNid + 2)
+  | .plus e1 e2 =>
+    let (e1, maxNid) := compileAux maxNid e1
+    let (e2, maxNid) := compileAux maxNid e2
+    let plusId := maxNid
+    let outId := maxNid + 1
+    let dfg := mergeTwo e1 e2 plusId
+    let dfg := ⟨plusId, .binOp .plus [⟨outId, 0⟩]⟩ :: ⟨outId, .output⟩ :: dfg
+    (⟨dfg, ⟨outId, 0⟩⟩, maxNid + 2)
+
+@[simp]
+def compile (e : Exp) : MarkedDFG :=
+  (compileAux 0 e).fst
+
+end Compiler
