Spacetalk/Correctness.lean
@@ -1,0 +1,347 @@
+import Aesop
+import Spacetalk.Compiler
+
+open Arith DF Compiler
+
+namespace DF
+
+  @[simp]
+  def Node.isOutput : Node → Bool
+    | ⟨_, .output⟩ => true
+    | _ => false
+
+end DF
+
+namespace Compiler.MarkedDFG
+
+  @[simp]
+  def initialState (dfg : MarkedDFG) (env : Env) : State :=
+    dfg.dfg.foldl
+      (λ state node =>
+        match node with
+        | ⟨nid, .input var _⟩ => state ↦ ⟨env var, ⟨nid, 0⟩⟩
+        | _ => state
+      )
+      .empty
+
+  @[simp]
+  def finalState (dfg : MarkedDFG) (val : Nat) : State :=
+    .empty ↦ ⟨val, dfg.ret⟩
+
+end Compiler.MarkedDFG
+
+lemma mergeTwo_nid_in_original : ∀ node ∈ mergeTwo g1 g2 newOutput, (∃ node' ∈ g1.dfg, node.id = node'.id) ∨ ∃ node' ∈ g2.dfg, node.id = node'.id := by
+  intro node h_mem
+  simp only [mergeTwo, removeOutputNodes, updateReturn, mergeVars, List.map_map, List.mem_filter,
+    List.mem_map, Function.comp_apply] at h_mem
+  obtain ⟨⟨node', ⟨h_mem', h_eq⟩⟩⟩ := h_mem
+  rw [←h_eq]
+  apply List.foldlRecOn g2.dfg mergeVarsAux g1.dfg _ _ _ h_mem'
+    (motive := λ dfg => ∀ node ∈ dfg,
+                          (∃ node', node' ∈ g1.dfg ∧ node.id = node'.id)
+                            ∨ (∃ node', node' ∈ g2.dfg ∧ node.id = node'.id))
+  · -- aesop?
+    rename_i right
+    intro node_1 a
+    subst h_eq
+    simp_all only
+    split at right
+    next x heq =>
+      split at heq
+      next x_1 var ports heq_1 =>
+        split at heq_1
+        next x_2 var_1 ports_1 heq_2 => simp_all only [Bool.false_eq_true]
+        next x_2 heq_2 => simp_all only [Bool.false_eq_true]
+        next x_2 op ports_1 heq_2 => simp_all only [Bool.false_eq_true]
+      next x_1 heq_1 =>
+        split at heq_1
+        next x_2 var ports heq_2 => simp_all only [Bool.false_eq_true]
+        next x_2 heq_2 => simp_all only [Bool.false_eq_true]
+        next x_2 op ports heq_2 => simp_all only [Bool.false_eq_true]
+      next x_1 op ports heq_1 =>
+        split at heq_1
+        next x_2 var ports_1 heq_2 => simp_all only [Bool.false_eq_true]
+        next x_2 heq_2 => simp_all only [Bool.false_eq_true]
+        next x_2 op_1 ports_1 heq_2 => simp_all only [Bool.false_eq_true]
+    next x x_1 =>
+      split at x_1
+      rename_i x_2 var ports heq
+      split at heq
+      rename_i x_3 var_1 ports_1 heq_1
+      simp_all only [reduceCtorEq, implies_true, NodeOp.input.injEq]
+      obtain ⟨left, right⟩ := heq
+      subst right left
+      apply Or.inl
+      apply Exists.intro
+      apply And.intro
+      on_goal 6 => rename_i x_2 heq
+      on_goal 7 => rename_i x_2 op ports heq
+      on_goal 4 => rename_i x_3 heq_1
+      on_goal 5 => rename_i x_3 op ports_1 heq_1
+      on_goal 6 => split at heq
+      on_goal 6 => rename_i x_3 var ports heq_1
+      on_goal 7 => rename_i x_3 heq_1
+      on_goal 8 => rename_i x_3 op ports heq_1
+      on_goal 9 => split at heq
+      on_goal 9 => rename_i x_3 var ports_1 heq_1
+      on_goal 10 => rename_i x_3 heq_1
+      on_goal 11 => rename_i x_3 op_1 ports_1 heq_1
+      on_goal 2 => {rfl
+      }
+      · simp_all only
+      simp_all only [NodeOp.input.injEq, true_and, imp_false, reduceCtorEq]
+      simp_all only [reduceCtorEq, implies_true]
+      simp_all only [imp_false, not_true_eq_false]
+      simp_all only [imp_false, not_true_eq_false]
+      simp_all only [imp_false, not_true_eq_false]
+      simp_all only [reduceCtorEq, implies_true]
+      simp_all only [NodeOp.binOp.injEq, true_and, imp_false, reduceCtorEq]
+      simp_all only [reduceCtorEq, implies_true, NodeOp.binOp.injEq, true_and]
+      subst heq
+      apply Or.inl
+      apply Exists.intro
+      · apply And.intro
+        on_goal 2 => {rfl
+        }
+        · simp_all only
+  · intro dfg ih node h_mem node' h_mem'
+    simp only [mergeVarsAux] at h_mem'
+    split at h_mem'
+    · split at h_mem'
+      · apply (List.mem_or_eq_of_mem_set h_mem').elim
+        · simp_all
+        · intro h
+          rw [h]
+          rename_i heq
+          have ⟨node, h⟩ := List.get?_eq_some_iff.mp heq
+          apply ih _ (List.mem_iff_get.mpr ⟨_, h⟩)
+      · -- aesop?
+        rename_i right node'_1 h_mem'_1 node_1 id var' a x x_1
+        subst h_eq
+        simp_all only [List.get?_eq_getElem?, imp_false, List.mem_cons]
+        cases h_mem' with
+        | inl h =>
+          subst h
+          simp_all only
+          split at right
+          next x_2 heq =>
+            split at heq
+            next x_3 var ports heq_1 =>
+              split at heq_1
+              next x_4 var_1 ports_1 heq_2 => simp_all only [Bool.false_eq_true]
+              next x_4 heq_2 => simp_all only [Bool.false_eq_true]
+              next x_4 op ports_1 heq_2 => simp_all only [Bool.false_eq_true]
+            next x_3 heq_1 =>
+              split at heq_1
+              next x_4 var ports heq_2 => simp_all only [Bool.false_eq_true]
+              next x_4 heq_2 => simp_all only [Bool.false_eq_true]
+              next x_4 op ports heq_2 => simp_all only [Bool.false_eq_true]
+            next x_3 op ports heq_1 =>
+              split at heq_1
+              next x_4 var ports_1 heq_2 => simp_all only [Bool.false_eq_true]
+              next x_4 heq_2 => simp_all only [Bool.false_eq_true]
+              next x_4 op_1 ports_1 heq_2 => simp_all only [Bool.false_eq_true]
+          next x_2 x_3 =>
+            split at x_3
+            next x_4 var ports heq =>
+              split at heq
+              next x_5 var_1 ports_1
+                heq_1 =>
+                simp_all only [reduceCtorEq, implies_true, NodeOp.input.injEq]
+                obtain ⟨left, right⟩ := heq
+                subst left right
+                apply Or.inr
+                apply Exists.intro
+                · apply And.intro
+                  · exact h_mem
+                  · simp_all only
+              next x_5 heq_1 => simp_all only [NodeOp.input.injEq, true_and, imp_false, reduceCtorEq]
+              next x_5 op ports_1 heq_1 => simp_all only [reduceCtorEq, implies_true]
+            next x_4 heq =>
+              split at heq
+              next x_5 var ports heq_1 => simp_all only [implies_true, imp_false, not_true_eq_false]
+              next x_5 heq_1 => simp_all only [implies_true, imp_false, not_true_eq_false]
+              next x_5 op ports heq_1 => simp_all only [implies_true, imp_false, not_true_eq_false]
+            next x_4 op ports heq =>
+              split at heq
+              next x_5 var ports_1 heq_1 => simp_all only [reduceCtorEq, implies_true]
+              next x_5 heq_1 => simp_all only [NodeOp.binOp.injEq, true_and, imp_false, reduceCtorEq]
+              next x_5 op_1 ports_1
+                heq_1 =>
+                simp_all only [reduceCtorEq, implies_true, NodeOp.binOp.injEq, true_and]
+                subst heq
+                apply Or.inr
+                apply Exists.intro
+                · apply And.intro
+                  · exact h_mem
+                  · simp_all only
+        | inr h_1 => simp_all only
+    · -- aesop?
+      rename_i right node'_1 h_mem'_1 node_2 x
+      subst h_eq
+      simp_all only [imp_false, List.mem_cons]
+      cases h_mem' with
+      | inl h =>
+        subst h
+        split at right
+        next x_1 heq =>
+          split at heq
+          next x_2 var ports heq_1 =>
+            split at heq_1
+            next x_3 var_1 ports_1 heq_2 => simp_all only [Bool.false_eq_true]
+            next x_3 heq_2 => simp_all only [Bool.false_eq_true]
+            next x_3 op ports_1 heq_2 => simp_all only [Bool.false_eq_true]
+          next x_2 heq_1 =>
+            split at heq_1
+            next x_3 var ports heq_2 => simp_all only [Bool.false_eq_true]
+            next x_3 heq_2 => simp_all only [Bool.false_eq_true]
+            next x_3 op ports heq_2 => simp_all only [Bool.false_eq_true]
+          next x_2 op ports heq_1 =>
+            split at heq_1
+            next x_3 var ports_1 heq_2 => simp_all only [Bool.false_eq_true]
+            next x_3 heq_2 => simp_all only [Bool.false_eq_true]
+            next x_3 op_1 ports_1 heq_2 => simp_all only [Bool.false_eq_true]
+        next x_1 x_2 =>
+          split at x_2
+          rename_i x_3 var ports heq
+          split at heq
+          rename_i x_4 var_1 ports_1 heq_1
+          simp_all only [reduceCtorEq, implies_true, NodeOp.input.injEq]
+          obtain ⟨left, right⟩ := heq
+          subst left right
+          apply Or.inr
+          apply Exists.intro
+          apply And.intro
+          on_goal 6 => rename_i x_3 heq
+          on_goal 7 => rename_i x_3 op ports heq
+          on_goal 4 => rename_i x_4 heq_1
+          on_goal 5 => rename_i x_4 op ports_1 heq_1
+          on_goal 6 => split at heq
+          on_goal 6 => rename_i x_4 var ports heq_1
+          on_goal 7 => rename_i x_4 heq_1
+          on_goal 8 => rename_i x_4 op ports heq_1
+          on_goal 9 => split at heq
+          on_goal 9 => rename_i x_4 var ports_1 heq_1
+          on_goal 10 => rename_i x_4 heq_1
+          on_goal 11 => rename_i x_4 op_1 ports_1 heq_1
+          on_goal 2 => {rfl
+          }
+          · simp_all only
+          simp_all only [NodeOp.input.injEq, true_and, imp_false, reduceCtorEq]
+          simp_all only [reduceCtorEq, implies_true]
+          simp_all only [imp_false, not_true_eq_false]
+          simp_all only [imp_false, not_true_eq_false]
+          simp_all only [imp_false, not_true_eq_false]
+          simp_all only [reduceCtorEq, implies_true]
+          simp_all only [NodeOp.binOp.injEq, true_and, imp_false, reduceCtorEq]
+          simp_all only [reduceCtorEq, implies_true, NodeOp.binOp.injEq, true_and]
+          subst heq
+          apply Or.inr
+          apply Exists.intro
+          · apply And.intro
+            on_goal 2 => {rfl
+            }
+            · simp_all only
+      | inr h_1 => simp_all only
+
+lemma maxNid_lt_new_maxNid : maxNid < (compileAux maxNid e).2 := by
+  cases e with
+  | var => aesop
+  | plus e1 e2 =>
+    simp only [compileAux]
+    have := maxNid_lt_new_maxNid (e := e1) (maxNid := maxNid)
+    have := maxNid_lt_new_maxNid (e := e2) (maxNid := (compileAux maxNid e1).2)
+    omega
+
+lemma nid_lt_new_maxNid : ∀ node ∈ (compileAux maxNid e).1.dfg, node.id < (compileAux maxNid e).2 := by
+  cases e with
+  | var => aesop
+  | plus e1 e2 =>
+    intro node h_mem
+    simp_all only [compileAux]
+    repeat (apply (List.mem_cons.mp h_mem).elim (by simp_all); intro h_mem)
+    apply (mergeTwo_nid_in_original _ h_mem).elim
+    <;> (intro h;
+         obtain ⟨node', ⟨h_mem, h_eq⟩⟩ := h;
+         rw [h_eq];
+         have := maxNid_lt_new_maxNid (e := e2) (maxNid := (compileAux maxNid e1).2);
+         have := nid_lt_new_maxNid _ h_mem;
+         omega)
+
+lemma output_if_ret
+  : ∀ node ∈ (compileAux maxNid e).1.dfg, node.id = (compileAux maxNid e).1.ret.node → node.isOutput = true := by
+  intro node h_mem h_ret
+  cases e with
+  | var => aesop
+  | plus e1 e2 =>
+    simp_all only [compileAux]
+    have :
+      ∀ node ∈ mergeTwo
+                (compileAux maxNid e1).fst
+                (compileAux (compileAux maxNid e1).snd e2).fst
+                (compileAux (compileAux maxNid e1).snd e2).snd,
+        node.id ≠ (compileAux (compileAux maxNid e1).snd e2).snd + 1 := by
+      intro node h_mem
+      apply (mergeTwo_nid_in_original _ h_mem).elim
+      <;> (intro h;
+           obtain ⟨node', ⟨h_mem, h_eq⟩⟩ := h;
+           have := nid_lt_new_maxNid _ h_mem;
+           have := maxNid_lt_new_maxNid (e := e2) (maxNid := (compileAux maxNid e1).2);
+           omega)
+    aesop
+
+lemma compile_value_correct (eval : Eval env e v)
+  : (compileAux maxNid e).1.dfg.MultiStep ((compileAux maxNid e).1.initialState env) ((compileAux maxNid e).1.finalState v) := by
+  cases e with
+  | var name =>
+    apply Relation.ReflTransGen.single
+    apply DFG.Step.node ⟨maxNid, .input name [⟨maxNid + 1, 0⟩]⟩
+    · simp
+    · refine Eq.subst ?_ (Node.Step.input ?_)
+      cases eval
+      aesop
+  | plus e1 e2 =>
+    cases eval
+    rename_i x y eval1 eval2
+    have ih1 := compile_value_correct eval1 (maxNid := maxNid)
+    have ih2 := compile_value_correct eval2 (maxNid := (compileAux maxNid e1).2)
+    sorry
+
+theorem compile_confluence {e : Exp} {a b c : State}
+  : (compile e).dfg.MultiStep a b → (compile e).dfg.MultiStep a c
+      → ∃ d, (compile e).dfg.MultiStep b d ∧ (compile e).dfg.MultiStep c d
+  | .refl, .refl => ⟨a, .intro .refl .refl⟩
+  | .refl, s => ⟨c, .intro s .refl⟩
+  | s, .refl => ⟨b, .intro .refl s⟩
+  | .tail gs1 ns1, .tail gs2 ns2 => by
+    cases ns1
+    cases ns2
+    rename_i _ _ b c node1 h_mem1 ns1 node2 h_mem2 ns2
+    rename_i c' b'
+    cases ns1 <;> cases ns2
+    all_goals sorry
+
+theorem final_state_halts {e : Exp} {v : Nat}
+  : ∀ s, (compile e).dfg.MultiStep ((compile e).finalState v) s → s = (compile e).finalState v := by
+  intro s step
+  induction step with
+  | refl => rfl
+  | tail _ step ih =>
+    rw [ih] at step
+    obtain ⟨⟨nid, op⟩, h_mem, step⟩ := step
+    cases step
+    <;> (have h_ret : ⟨nid, 0⟩ = (compile e).ret := by simp_all;
+         have := output_if_ret _ h_mem (Port.mk.inj h_ret).left;
+         simp at this)
+
+theorem compile_correct {e : Exp} {env : Env} {v : Nat}
+  : Eval env e v
+    → ∀ s, (compile e).dfg.MultiStep ((compile e).initialState env) s
+          → (compile e).dfg.MultiStep s ((compile e).finalState v) := by
+  intro as s ds
+  have := compile_confluence ds (compile_value_correct as)
+  obtain ⟨w, h⟩ := this
+  obtain ⟨left, right⟩ := h
+  have := final_state_halts w right
+  rw [this] at left
+  exact left
