Spacetalk/DF.lean
@@ -1,0 +1,80 @@
+import Mathlib.Logic.Relation
+
+namespace DF
+
+-- Syntax
+structure Port where
+  node : Nat
+  port : Nat
+deriving DecidableEq
+
+inductive BinOp
+  | plus
+
+inductive NodeOp
+  | input : String → List Port → NodeOp
+  | output : NodeOp
+  | binOp : BinOp → List Port → NodeOp
+
+structure Node where
+  id : Nat
+  op : NodeOp
+
+abbrev DFG := List Node
+
+-- Semantics
+abbrev State := Port → List Nat
+
+structure Token where
+  val : Nat
+  port : Port
+
+structure BToken where
+  val : Nat
+  ports : List Port
+
+@[simp]
+def State.empty : State := λ _ => []
+
+@[simp]
+def State.pop (s : State) (p : Port) : State :=
+  λ p' => if p' = p then (s p).tail else s p'
+
+@[simp]
+def State.push (s : State) (tok : Token) : State :=
+  λ p => if p = tok.port then (s tok.port).concat tok.val else (s p)
+
+@[simp]
+def State.pushAll (s : State) (tok : BToken) : State :=
+  tok.ports.foldl (λ s port => s.push ⟨tok.val, port⟩) s
+
+@[simp]
+def BinOp.denote : BinOp → Nat → Nat → Nat
+  | plus => HAdd.hAdd
+
+infixl:100 " ↤ " => State.pop
+infixl:100 " ↦ " => State.push
+infixl:100 " ↦↦ " => State.pushAll
+
+inductive Node.Step : Node → State → State → Prop
+  | input : (h : s ⟨nid, 0⟩ ≠ [])
+    → Node.Step ⟨nid, .input var ports⟩
+      s
+      (s
+        ↤ ⟨nid, 0⟩
+        ↦↦ ⟨(s ⟨nid, 0⟩).head h, ports⟩)
+  | binOp : {op : BinOp} → (h1 : s ⟨nid, 0⟩ ≠ []) → (h2 : s ⟨nid, 1⟩ ≠ [])
+    → Node.Step ⟨nid, .binOp op ports⟩
+      s
+      (s
+        ↤ ⟨nid, 0⟩
+        ↤ ⟨nid, 1⟩
+        ↦↦ ⟨op.denote ((s ⟨nid, 0⟩).head h1) ((s ⟨nid, 1⟩).head h2), ports⟩)
+
+inductive DFG.Step : DFG → State → State → Prop
+  | node : (node : Node) → node ∈ dfg → node.Step s1 s2 → DFG.Step dfg s1 s2
+
+abbrev DFG.MultiStep (dfg : DFG) : State → State → Prop :=
+  Relation.ReflTransGen dfg.Step
+
+end DF
